

$$1) BA = \begin{bmatrix} -3 & -2 & 0 \\ -2 & 3 & 0 \\ 0 & 0 & 5 \end{bmatrix} \begin{bmatrix} 4 & 0 & 1 \\ -2 & 1 & 0 \\ -2 & 0 & 1 \end{bmatrix}$$

$$\begin{aligned} \text{Baris 1} &= 3(4) + (-2)(-2) + 0(-2) = 14 \\ &= 3(0) + (-2)(1) + 0(0) = -2 \\ &= 3(1) + (-2)(0) + 0(1) = 3 \end{aligned}$$

$$\text{Baris 2} = \begin{matrix} -14 \\ 3 \\ -2 \end{matrix}$$

$$\text{Baris 3} = \begin{matrix} -10 \\ 0 \\ 5 \end{matrix} \quad BA = \begin{bmatrix} 16 & -2 & 3 \\ -14 & 3 & -2 \\ -10 & 0 & 5 \end{bmatrix}$$

$$B^T A^T = (AB)^T$$

$$AB = \begin{bmatrix} 4 & 0 & 1 \\ -2 & 1 & 0 \\ -2 & 0 & 1 \end{bmatrix}$$

$$\begin{bmatrix} 3 & -2 & 0 \\ -2 & 3 & 0 \\ 0 & 0 & 5 \end{bmatrix}$$

$$AB = \begin{bmatrix} 12 & -8 & 5 \\ -8 & 7 & 0 \\ -6 & 4 & 5 \end{bmatrix}$$

$$(AB)^T = \begin{bmatrix} 12 & -8 & -6 \\ -8 & 7 & 0 \\ 5 & 0 & 5 \end{bmatrix}$$

$$I + BA - B^T A^T$$

$$I = \begin{bmatrix} 1 & 0 & 0 \\ 0 & 1 & 0 \\ 0 & 0 & 1 \end{bmatrix} = \begin{bmatrix} 1 & 0 & 0 \\ 0 & 1 & 0 \\ 0 & 0 & 1 \end{bmatrix} + \begin{bmatrix} 16 & -3 & 3 \\ -7 & 3 & -2 \\ -10 & 0 & 7 \end{bmatrix} - \begin{bmatrix} 12 & -8 & -6 \\ 8 & 7 & 4 \\ 0 & 0 & 5 \end{bmatrix}$$

$$= \begin{bmatrix} 5 & 6 & 9 \\ -6 & -3 & -6 \\ -15 & 0 & 1 \end{bmatrix}$$

$$2) \begin{bmatrix} 5 & 4 \\ 1 & 8 \end{bmatrix} - \begin{bmatrix} 3 & 5 \\ 4 & 6 \end{bmatrix} = \begin{bmatrix} 2 & -1 \\ -3 & 2 \end{bmatrix}$$

$$B \leftarrow A - C$$

$$\begin{bmatrix} 2 & -1 \\ 4 & 6 \end{bmatrix} = \begin{bmatrix} 5 & 4 \\ 1 & 8 \end{bmatrix} - \begin{bmatrix} 3 & 5 \\ 4 & 6 \end{bmatrix}$$

$$\begin{bmatrix} 2 & -1 \\ 4 & 6 \end{bmatrix} = \begin{bmatrix} 2 & -1 \\ 4 & 6 \end{bmatrix} \Rightarrow \text{jadi } B \times 2 = B$$

$$C = A - B \text{ baru}$$

$$3) R_2 \leftarrow R_2 - 2R_1$$

$$R_3 \leftarrow R_3 - 3R_1$$

$$R_2 = [2, 4, -2, 6] - 2[1, 3, 1, 4] = [0, -2, -4, 2]$$

$$R_3 = [3, 7, 5, 8] - 3[1, 3, 1, 4] = [0, -2, 2, -4]$$

$$\begin{bmatrix} 1 & 3 & 1 & 4 \\ 0 & -2 & -4 & 2 \\ 0 & -2 & 2 & -4 \end{bmatrix}$$



$$R_2 \leftarrow \frac{1}{2} R_2 = [0, 1, 2, 1]$$

$$R_1 \leftarrow R_1 - 3R_2 = [1, 0, -7, 1]$$

$$R_3 \leftarrow R_3 - 2R_2 = [0, 0, 6, -2]$$

$$\begin{bmatrix} 1 & 0 & -7 & 1 \\ 0 & 1 & 2 & 1 \\ 0 & 0 & 6 & -2 \end{bmatrix}$$

$$R_3 \leftarrow \frac{1}{6} R_3 = [0, 0, 1, -1/3]$$

$$\begin{bmatrix} 1 & 0 & -7 & 1 \\ 0 & 1 & 2 & 1 \\ 0 & 0 & 1 & -1/3 \end{bmatrix}$$

4)

5) Mencari  $P^{-1}$  dengan cara  $[P | I]$

$$P = \begin{bmatrix} 3 & 1 & -2 \\ 7 & -2 & -3 \\ 2 & 2 & 3 \end{bmatrix} \quad I = \begin{bmatrix} 1 & 0 & 0 \\ 0 & 1 & 0 \\ 0 & 0 & 1 \end{bmatrix}$$

$$\Rightarrow P^{-1} = \frac{1}{99} \begin{bmatrix} 0 & 7 & 7 \\ 21 & -13 & 1 \\ 14 & 4 & 11 \end{bmatrix}$$

$$= \begin{bmatrix} 0 & 1/7 & 1/7 \\ 3/7 & -13/99 & 1/99 \\ -2/7 & 4/99 & 11/99 \end{bmatrix}$$